@prefix : <http://purl.org/net/opmv/ns#> .
@prefix ns: <http://purl.org/net/opmv/ns#> .
@prefix owl: <http://www.w3.org/2002/07/owl#> .
@prefix rdf: <http://www.w3.org/1999/02/22-rdf-syntax-ns#> .
@prefix www: <http://www.jenitennison.com/#> .
@prefix xml: <http://www.w3.org/XML/1998/namespace> .
@prefix xsd: <http://www.w3.org/2001/XMLSchema#> .
@prefix foaf: <http://xmlns.com/foaf/0.1/> .
@prefix opmv: <http://purl.org/net/opmv/> .
@prefix rdfs: <http://www.w3.org/2000/01/rdf-schema#> .
@prefix time: <http://www.w3.org/2006/time#> .
@prefix void: <http://rdfs.org/ns/void#> .
@prefix terms: <http://purl.org/dc/terms/> .
@prefix owl2xml: <http://www.w3.org/2006/12/owl2-xml#> .
@base <http://purl.org/net/opmv/ns> .

<http://purl.org/net/opmv/ns> rdf:type owl:Ontology .

#################################################################
#    Datatypes
#################################################################

###  http://www.w3.org/2001/XMLSchema#date
xsd:date rdf:type rdfs:Datatype .


#################################################################
#    Object Properties
#################################################################

###  http://purl.org/dc/terms/creator
terms:creator rdf:type owl:ObjectProperty .


###  http://purl.org/net/opmv/used
opmv:used rdf:type owl:ObjectProperty ;
          rdfs:domain opmv:Process ;
          rdfs:range opmv:Artifact ;
          rdfs:comment "used is an abstract property to express that a process used an artifact"@en ;
          rdfs:isDefinedBy <http://purl.org/net/opmv/ns> .


###  http://purl.org/net/opmv/wasControlledBy
opmv:wasControlledBy rdf:type owl:ObjectProperty ;
                     rdfs:domain opmv:Process ;
                     rdfs:range opmv:Agent ;
                     rdfs:comment "wasControlledBy is an abstract property to express that a process was controlled by an agent."@en ;
                     rdfs:isDefinedBy <http://purl.org/net/opmv/ns> .


###  http://purl.org/net/opmv/wasDerivedFrom
opmv:wasDerivedFrom rdf:type owl:ObjectProperty ;
                    rdfs:domain opmv:Artifact ;
                    rdfs:range opmv:Artifact ;
                    rdfs:comment "wasDerivedFrom is an abstract property to express that an artifact was derived from another artifact."@en ;
                    rdfs:isDefinedBy <http://purl.org/net/opmv/ns> .


###  http://purl.org/net/opmv/wasEncodedBy
opmv:wasEncodedBy rdf:type owl:ObjectProperty ;
                  rdfs:subPropertyOf opmv:wasDerivedFrom ;
                  rdfs:domain opmv:Artifact ;
                  rdfs:range opmv:Artifact ;
                  rdfs:comment "wasEncodedBy is an object property to express that an artifact is encoded by another artifact. The property is useful for expressing the relationship between the data and the file encoding the data."@en ;
                  rdfs:isDefinedBy <http://purl.org/net/opmv/ns> .


###  http://purl.org/net/opmv/wasEndedAt
opmv:wasEndedAt rdf:type owl:ObjectProperty ;
                rdfs:domain opmv:Process ;
                rdfs:range time:Instant ;
                owl:propertyChainAxiom ( opmv:wasPerformedAt
                                         time:hasEnd
                                       ) ;
                rdfs:comment "wasEndedAt is an object property to express that a process was finished at a specific time instant. The property chain defines that all processes, that were performed during a specific time period which ended at a specific instant, were actually finished at that specific time instant."@en ;
                rdfs:isDefinedBy <http://purl.org/net/opmv/ns> .


###  http://purl.org/net/opmv/wasGeneratedAt
opmv:wasGeneratedAt rdf:type owl:ObjectProperty ;
                    rdfs:subPropertyOf owl:topObjectProperty ;
                    rdfs:domain opmv:Artifact ;
                    rdfs:range time:Instant ;
                    rdfs:comment "wasGeneratedAt is an object property to express that an artifact was generated at a specific time instant. This property is very similar to dct:created. Note that in a very fine-grained case the time when an artifact was generated might not be the same as the time when the process producing that artifact finished."@en ;
                    rdfs:isDefinedBy <http://purl.org/net/opmv/ns> .


###  http://purl.org/net/opmv/wasGeneratedBy
opmv:wasGeneratedBy rdf:type owl:ObjectProperty ;
                    rdfs:domain opmv:Artifact ;
                    rdfs:range opmv:Process ;
                    rdfs:comment "wasGeneratedBy is an abstract property to express that an artifact was generated by a process."@en ;
                    rdfs:isDefinedBy <http://purl.org/net/opmv/ns> .


###  http://purl.org/net/opmv/wasPerformedAt
opmv:wasPerformedAt rdf:type owl:ObjectProperty ;
                    rdfs:subPropertyOf owl:topObjectProperty ;
                    rdfs:domain opmv:Process ;
                    rdfs:range time:TemporalEntity ;
                    rdfs:comment "wasPerformedAt is an object property to express that a process is performed either at a specific time instant or during a specific time interval."@en ;
                    rdfs:isDefinedBy <http://purl.org/net/opmv/ns> .


###  http://purl.org/net/opmv/wasPerformedBy
opmv:wasPerformedBy rdf:type owl:ObjectProperty ;
                    rdfs:subPropertyOf opmv:wasControlledBy ;
                    rdfs:domain opmv:Process ;
                    rdfs:range opmv:Agent ;
                    rdfs:comment "wasPerformedBy is an object property to express that a process was performed by another process. It is a sub-property of wasControlledBy."@en ;
                    rdfs:isDefinedBy <http://purl.org/net/opmv/ns> .


###  http://purl.org/net/opmv/wasStartedAt
opmv:wasStartedAt rdf:type owl:ObjectProperty ;
                  rdfs:domain opmv:Process ;
                  rdfs:range time:Instant ;
                  owl:propertyChainAxiom ( opmv:wasPerformedAt
                                           time:hasBeginning
                                         ) ;
                  rdfs:comment "wasStartedAt is an object property to express that a process is started at a specific time instant. The property chain defines that all processes, that were performed during a specific time period which began at a specific instant, were actually started at that specific time instant."@en ;
                  rdfs:isDefinedBy <http://purl.org/net/opmv/ns> .


###  http://purl.org/net/opmv/wasTriggeredBy
opmv:wasTriggeredBy rdf:type owl:ObjectProperty ;
                    rdfs:domain opmv:Process ;
                    rdfs:range opmv:Process ;
                    rdfs:comment "wasTriggeredBy is an abstract property to express that a process was triggerred by another process."@en ;
                    rdfs:isDefinedBy <http://purl.org/net/opmv/ns> .


###  http://purl.org/net/opmv/wasUsedAt
opmv:wasUsedAt rdf:type owl:ObjectProperty ;
               rdfs:subPropertyOf owl:topObjectProperty ;
               rdfs:domain opmv:Artifact ;
               rdfs:range time:Instant ;
               rdfs:comment "wasUsedAt is an object property to express that an artifact was used at a specific time instant. An artifact might not be used at the starting time of the process that actually consumed it. Hence, we provide a different time-related property to express when an artifact was used."@en ;
               rdfs:isDefinedBy <http://purl.org/net/opmv/ns> .


###  http://purl.org/net/opmv/withRespectOf
opmv:withRespectOf rdf:type owl:ObjectProperty ;
                   rdfs:subPropertyOf owl:topObjectProperty ;
                   rdfs:domain time:Instant ;
                   rdfs:range opmv:Process ;
                   rdfs:comment "withRespectOf is an object property to associate a time instant at which an artifact was used or generated with the process that used or generated that artifact. At a very fine-grained distinction, the time when an artifact was used or generated might not be exactly the same as the starting or ending time of the process in which the artifact was involved. The related properties opmv:wasUsedAt and opmv:wasGeneratedAt can be used as shortcuts to express time-related information about an artifact. The property opmv:wasUsedAt is only used when users want to express precisely in which process an artifact was used or generated. It can be omitted in most cases."@en ;
                   rdfs:isDefinedBy <http://purl.org/net/opmv/ns> .


###  http://rdfs.org/ns/void#exampleResource
void:exampleResource rdf:type owl:ObjectProperty .


###  http://www.w3.org/2002/07/owl#topObjectProperty
owl:topObjectProperty rdf:type owl:ObjectProperty .


###  http://www.w3.org/2006/time#hasBeginning
time:hasBeginning rdf:type owl:ObjectProperty ;
                  rdfs:domain time:TemporalEntity ;
                  rdfs:range time:Instant ;
                  rdfs:isDefinedBy "http://www.w3.org/2006/time"^^xsd:anyURI .


###  http://www.w3.org/2006/time#hasEnd
time:hasEnd rdf:type owl:ObjectProperty ;
            rdfs:domain time:TemporalEntity ;
            rdfs:range time:Instant ;
            rdfs:isDefinedBy "http://www.w3.org/2006/time"^^xsd:anyURI .


#################################################################
#    Data properties
#################################################################

###  http://purl.org/dc/terms/created
terms:created rdf:type owl:DatatypeProperty .


###  http://purl.org/dc/terms/modified
terms:modified rdf:type owl:DatatypeProperty .


###  http://purl.org/dc/terms/title
terms:title rdf:type owl:DatatypeProperty .


#################################################################
#    Classes
#################################################################

###  http://purl.org/net/opmv/Agent
opmv:Agent rdf:type owl:Class ;
           owl:equivalentClass foaf:Agent ;
           owl:disjointWith opmv:Process ;
           rdfs:comment "Agent is a contextual entity acting as a catalyst of a process, enabling, facilitating, controlling, or affecting its execution."@en ;
           rdfs:isDefinedBy <http://purl.org/net/opmv/ns> .


###  http://purl.org/net/opmv/Artifact
opmv:Artifact rdf:type owl:Class ;
              owl:disjointWith opmv:Process ;
              rdfs:comment "Artifact is a general concept that represents immutable piece of state, which may have a physical embodiment in a physical object, or a digital representation in a computer system."@en ;
              rdfs:isDefinedBy <http://purl.org/net/opmv/ns> .


###  http://purl.org/net/opmv/Process
opmv:Process rdf:type owl:Class .


###  http://rdfs.org/ns/void#Dataset
void:Dataset rdf:type owl:Class .


###  http://www.w3.org/2002/07/owl#Thing
owl:Thing rdf:type owl:Class .


###  http://www.w3.org/2006/time#Instant
time:Instant rdf:type owl:Class ;
             rdfs:subClassOf time:TemporalEntity ;
             rdfs:isDefinedBy "http://www.w3.org/2006/time"^^xsd:anyURI .


###  http://www.w3.org/2006/time#Interval
time:Interval rdf:type owl:Class ;
              rdfs:subClassOf time:TemporalEntity ;
              rdfs:isDefinedBy "http://www.w3.org/2006/time"^^xsd:anyURI .


###  http://www.w3.org/2006/time#TemporalEntity
time:TemporalEntity rdf:type owl:Class ;
                    rdfs:isDefinedBy "http://www.w3.org/2006/time"^^xsd:anyURI .


###  http://xmlns.com/foaf/0.1/Agent
foaf:Agent rdf:type owl:Class .


###  http://xmlns.com/foaf/0.1/Document
foaf:Document rdf:type owl:Class .


#################################################################
#    Individuals
#################################################################

###  http://purl.org/net/opmv/Process
opmv:Process rdf:type owl:NamedIndividual ,
                      owl:Thing .


###  http://purl.org/net/opmv/ns
<http://purl.org/net/opmv/ns> rdf:type owl:NamedIndividual ,
                                       void:Dataset ,
                                       owl:Thing ,
                                       foaf:Document ;
                              terms:creator www:me ;
                              void:exampleResource opmv:Process ;
                              terms:created "2010-04-14"^^xsd:date ;
                              terms:modified "2010-10-04"^^xsd:date ;
                              terms:title "The Core OPMV Vocabulary"@en .


###  http://www.jenitennison.com/#me
www:me rdf:type owl:NamedIndividual ,
                owl:Thing .


#################################################################
#    Annotations
#################################################################

opmv:Process rdfs:comment "Process refers to an action or series of actions performed on or caused by artifacts, and resulting in new artifacts."@en ;
             rdfs:isDefinedBy <http://purl.org/net/opmv/ns> .


###  Generated by the OWL API (version 4.5.9.2019-02-01T07:24:44Z) https://github.com/owlcs/owlapi
